got GrowPreservesAcyclic working again

disk-betree/DiskBetree.dfy
@@ -38,18 +38,35 @@ abstract module DiskBetree {
     && (forall k :: k !in node.children ==> BufferIsDefining(node.buffer[k]))
   }
 
-  predicate {:opaque} LookupFollowsChildRefs(key: Key, lookup: Lookup) {
-    && (forall i :: 0 <= i < |lookup| - 1 ==> IMapsTo(lookup[i].node.children, key, lookup[i+1].ref))
-  }
-  
-  lemma LookupFollowsChildRefsAtLayer(key: Key, lookup: Lookup, i: int)
-    requires LookupFollowsChildRefs(key, lookup)
-    requires 0 <= i < |lookup| - 1
-    ensures IMapsTo(lookup[i].node.children, key, lookup[i+1].ref)
+  predicate LookupFollowsChildRefsAtLayer(key: Key, lookup: Lookup, i: int)
+    requires 0 <= i < |lookup|-1
   {
-    reveal_LookupFollowsChildRefs();
+    IMapsTo(lookup[i].node.children, key, lookup[i+1].ref)
   }
   
+  predicate LookupFollowsChildRefs<Value>(key: Key, lookup: Lookup)
+    ensures |lookup| == 0 ==>  LookupFollowsChildRefs<Value>(key, lookup)
+  {
+    && (forall i :: 0 <= i < |lookup| - 1 ==> LookupFollowsChildRefsAtLayer(key, lookup, i))
+  }
+
+  lemma LookupFollowsChildRefsExtract(key: Key, lookup: Lookup, i: int)
+  //   requires LookupFollowsChildRefs(key, lookup)
+  //   requires 0 <= i < |lookup| - 1
+  //   ensures LookupFollowsChildRefsAtLayer(key, lookup, i)
+  // {
+  //   //reveal_LookupFollowsChildRefs();
+  // }
+
+  lemma LookupFollowsChildRefsAppend(key: Key, lookup: Lookup)
+  //   requires 0 < |lookup|
+  //   requires 1 < |lookup| ==> LookupFollowsChildRefsAtLayer(key, lookup, |lookup|-2)
+  //   requires LookupFollowsChildRefs(key, DropLast(lookup))
+  //   ensures LookupFollowsChildRefs(key, lookup)
+  // {
+  //   //reveal_LookupFollowsChildRefs();
+  // }
+    
   predicate LookupRespectsDisk<Value>(view: BI.View<Node<Value>>, lookup: Lookup) {
     forall i :: 0 <= i < |lookup| ==> IMapsTo(view, lookup[i].ref, lookup[i].node)
   }
